SHEET7
#+SETUPFILE: options.org
# Useful symbols, \circ, \bigsqcup

* Exercise 1
  For the definition of continuous functions
  $\bigsqcup f (s) = f(\bigsqcup s)$ and $\bigsqcup g (s) = g(\bigsqcup s)$
  \newline
  We want to prove that also:
  $g \circ f : D1 \rightarrow D3$ is also continuous.

  \newline
  In other words we want to prove that:
  $\bigsqcup g (f (s)) = g (f (\bigsqcup s))$
  We use the following chain of equivalences:
  - $\bigsqcup g(f (s)) = g (\bigsqcup f (s))$  -- applying continuity of g
  - $g (\bigsqcup f (s)) = g (f (\bigsqcup s))$ -- applying continuity of f

* Exercise 2
  Let $S \sqsubseteq \langle \mathbb{Z} \rightarrow \mathbb{Z} \rangle$ be a chain of continuous functions $S = {g1, g2, g3, ...}$

** (a) \phi_{sum} is monotonic
   \phi_{sum} is monotonic then $g1 \sqsubseteq g2 \rightarrow \phi_{sum}(g1) \sqsubseteq \phi_{sum}(g2)$
   
*** Case 1: x is \bot
    $\phi_{sum}(g1))(\bot) = (\phi_{sum}(g2))(\bot) =$
    \left \{
    \begin{array}{ll}
    \mbox{1 if  x <= 0} \\
    \bot \mbox{ otherwise}
    \end{array}
    \right
    
    So, \phi_{sum} is as defined as \phi_{sum}(g2).

*** Case 2: x \in \mathbb{\mathbb{Z}}
    \phi_{sum}(g1)(x) =
    \left \{
    \begin{array}{ll}
    \mbox{1, if x <= 0} \\
    g1(x-1) + x, \mbox{otherwise} \\
    \end{array}
    \right

    \phi_{sum}(g2)(x) =
    \left \{
    \begin{array}{ll}
    \mbox{1, if x <= 0} \\
    g2(x-1) + x, \mbox{otherwise} \\
    \end{array}
    \right

    $\phi_{sum}(g1) \sqsubseteq \phi_{sum}(g2)$ because $(g1(x - 1) + x) \sqsubseteq (g2(x - 1) + x)$ \newline

    Therefore, \phi_{sum} is *monotonic*.
    
** (b) \phi_{sum} is continuous
   If \phi_{sum} is continuous, then \bigsqcup \phi_{sum}(S) = \phi_{sum}(\bigsqcup S) and \phi_{sum} is monotonic.
   Let /g/ be the /LUB/ of S, \bigsqcup S = g

*** 1)
    \phi_{sum}(\bigsqcup S)(x) = \phi_{sum}(g)(x) =
    \left \{
    \begin{array}{ll}
    1, \mbox{if x <= 0} \\
    g(x - 1) + x, \mbox{otherwise} \\
    \end{array}
    \right

*** 2)
    \phi_{sum}(S) = {\phi_{sum}(g1), \phi_{sum}(g2)...} =
    \left \{
    \begin{array}{ll}
    \left \{
    \begin{array}{ll}
    1, \mbox{if x <= 0} \\
    g1(x - 1) + x, \mbox{otherwise} \\
    \end{array}
    \\
    \right
    \left \{
    \begin{array}{ll}
    1, \mbox{if x <= 0} \\
    g2(x - 1) + x, \mbox{otherwise} \\
    \end{array}
    \right
    \\
    \vdots
    \end{array}
    \right


    \phi_{sum}(S) = {\phi_{sum}(g1), \phi_{sum}(g2)...} =
    \bigsqcup \left \{
    \begin{array}{ll}
    \left \{
    \begin{array}{ll}
    1, \mbox{if x <= 0} \\
    g1(x - 1) + x, \mbox{otherwise} \\
    \end{array}
    \\
    \right
    \left \{
    \begin{array}{ll}
    1, \mbox{if x <= 0} \\
    g2(x - 1) + x, \mbox{otherwise} \\
    \end{array}
    \right
    \\
    \vdots
    \end{array}
    \right =

    \left \{
    \begin{array}{ll}
    1, \mbox{if x <= 0} \\
    g(x - 1) + x, \mbox{otherwise} \\
    \end{array}
    \right

    \newline \newline

    Since $\bigsqcup \phi_{sum}(S) = \phi_{sum}(\bigsqcup S)$ we can finally deduce that \phi_{sum} is continuous.

* Exercise 3

** (a) give the Haskell definitions for the higher order functions *f\_four*, *f\_inf* and *f\_times*
  

#+BEGIN_SRC haskell 
   f_four = \g -> \x -> 4

   f_inf  = \g -> \x -> g (x + 4)
   f_times = \g -> \(x, y) -> if x <= 0
                               then 0
                               else y + g(x - 1, y)
#+END_SRC


** (b) give the semantics of \phi_{f\_four}
   - (\phi_(f\_four)(g))(x) = 4
   - (\phi_(f\_inf)(g))(x) = g(x + 4)
   - (\phi_{f\_times}(g))(x, y) =
     \left \{
     \begin{array}{ll}
     0, \mbox{if x <= 0} \\
     y + g(x -1, y), \mbox{otherwise}\\
     \end{array}
     \right
   
** (c)
   - \phi^n{f\_four}(\bot) = 4 \newline
   - \phi^n{f\_inf}(\bot) = \bot \newline
   - \phi^n{f\_times}(\bot) =
     \left \{
     \begin{array}{ll}
     0, \mbox{if x <= 0} \\
     \bot, \mbox{otherwise}\\
     \end{array}
     \right

** (d) Give all fixpoints of the semantic functions \phi_{f\_four}, \phi_{f\_inf}, and \phi_{f\_times}. Which are /lub/?
   - fp(\phi_{f\_four}) = \tau_4(x) where \tau_4(x) = 4 \newline
     lfp(\phi_{f\_four}) = \tau_4(x) where \tau_4(x) = 4

   - fp(\phi_{f\_inf}) = { \tau_i(x) where \tau_i(x) = i | i \in \mathbb{R} \cup {\bot}} } \newline
     lfp(\phi_{f\_inf}) = \tau_i(x) where \tau_i(x) = \bot

     \newline
     \newline

   - fp(\phi_{f\_times}) = f(x y) where f(x,y) =
     \left \{
     \begin{array}{ll}
     0, \mbox{if x <= 0} \\
     x y, \mbox{if x > 0} \\
     \bot, \mbox{otherwise}\\
     \end{array}
     \right
     
     \newline
     lfp(\phi_{f\_times}) = f(x, y) where \newline
     f(x, y) =
     \left \{
     \begin{array}{ll}
     0, \mbox{if x <= 0} \\
     x y, \mbox{if x > 0} \\
     \bot, \mbox{otherwise} \\
     \end{array}
     \right
